Misc

isabelle-thys/Programs.thy
@@ -38,6 +38,7 @@ datatype raw_program =
   | QuantumOp \<open>(qu ell2, qu ell2, unit) kraus_family expression\<close>
   | Measurement \<open>(cl, qu) measurement expression\<close>
   | InstantiateOracles \<open>raw_program\<close> \<open>raw_program list\<close>
+     \<comment> \<open>\<^term>\<open>InstantiateOracles p q\<close> replace the first oracles in p by q, and decrease the index of all other oracle calls by len q.\<close>
   | LocalQ \<open>qu QREGISTER\<close> \<open>(qu ell2, qu ell2) trace_class\<close> \<open>raw_program\<close>
   | LocalC \<open>cl CREGISTER\<close> \<open>cl\<close> \<open>raw_program\<close>
       \<comment> \<open>Interpretation: \<^term>\<open>LocalC F init P\<close> temporarily back up the content of reference F,
@@ -52,7 +53,7 @@ fun oracle_number :: \<open>raw_program \<Rightarrow> nat\<close> where
 | \<open>oracle_number (Measurement _) = 0\<close>
 | \<open>oracle_number (IfThenElse e c d) = max (oracle_number c) (oracle_number d)\<close>
 | \<open>oracle_number (While e c) = oracle_number c\<close>
-| \<open>oracle_number (InstantiateOracles _ _) = 0\<close>
+| \<open>oracle_number (InstantiateOracles p qs) = max (oracle_number p - length qs) (\<Squnion>q\<in>set qs. oracle_number q)\<close>
 | \<open>oracle_number (LocalQ _ _ c) = oracle_number c\<close>
 | \<open>oracle_number (LocalC _ _ c) = oracle_number c\<close>
 | \<open>oracle_number (OracleCall i) = Suc i\<close>
@@ -66,6 +67,215 @@ fun no_oracles :: \<open>raw_program \<Rightarrow> bool\<close> where
 | \<open>no_oracles (OracleCall _) \<longleftrightarrow> False\<close>
 | \<open>no_oracles (InstantiateOracles _ _) \<longleftrightarrow> False\<close>
 | \<open>no_oracles p \<longleftrightarrow> True\<close>
+
+fun substitute_oracles_raw :: \<open>raw_program list \<Rightarrow> raw_program \<Rightarrow> raw_program\<close> where
+\<open>substitute_oracles_raw os (Seq c d) = Seq (substitute_oracles_raw os c) (substitute_oracles_raw os d)\<close>
+| \<open>substitute_oracles_raw os (IfThenElse e c d) = IfThenElse e (substitute_oracles_raw os c) (substitute_oracles_raw os d)\<close>
+| \<open>substitute_oracles_raw os (While e c) = While e (substitute_oracles_raw os c)\<close>
+| \<open>substitute_oracles_raw os (LocalQ Q \<rho> c) = LocalQ Q \<rho> (substitute_oracles_raw os c)\<close>
+| \<open>substitute_oracles_raw os (LocalC C m c) = LocalC C m (substitute_oracles_raw os c)\<close>
+| \<open>substitute_oracles_raw os (OracleCall i) = (if i < length os then os!i else OracleCall (i - length os))\<close>
+| \<open>substitute_oracles_raw os (InstantiateOracles c ds) = substitute_oracles_raw (map (substitute_oracles_raw os) ds @ os) c\<close>
+| \<open>substitute_oracles_raw os p = p\<close>
+
+lemma max_diff_distrib_left_nat: "max x y - z = max (x - z) (y - z)" for x y z :: nat
+  by (simp add: max_def)
+
+(* lemma cSUP_mono_simple: "bdd_above (g ` A) \<Longrightarrow> (\<And>n. n \<in> A \<Longrightarrow> f n \<le> g n) \<Longrightarrow> \<Squnion>(f ` A) \<le> \<Squnion>(g ` A)"
+  for f g :: \<open>_ \<Rightarrow> _::conditionally_complete_lattice\<close>
+  apply (cases \<open>A = {}\<close>)
+apply (simp add: )
+try0
+sledgehammer [dont_slice]
+by -
+ *)
+
+lemma [iff]: \<open>is_Sup {} (\<bottom>::_::order_bot)\<close>
+  by (simp add: is_Sup_def)
+
+
+lemma OFCLASS_conditionally_complete_lattice_Sup_orderI:
+  assumes \<open>Sup {} = (\<bottom>::'a)\<close>
+  shows \<open>OFCLASS('a::{conditionally_complete_lattice, order_bot}, Sup_order_class)\<close>
+proof
+  show \<open>is_Sup X (\<Squnion> X)\<close> if \<open>has_Sup X\<close> for X :: \<open>'a set\<close>
+  proof (cases \<open>X = {}\<close>)
+    case True
+    then show ?thesis
+      by (simp add: assms)
+  next
+    case False
+    with that show ?thesis
+      by (auto intro!: is_Sup_cSup has_Sup_bdd_above simp: )
+  qed
+  show \<open>is_Sup {x, y} (x \<squnion> y)\<close> if \<open>has_Sup {x, y}\<close> for x y :: 'a
+  by (simp add: is_Sup_def)
+qed
+
+instance nat :: Sup_order
+  apply (rule OFCLASS_conditionally_complete_lattice_Sup_orderI)
+  by (simp add: bot_nat_def)
+
+lemma (in Sup_order) Sup_eqI:
+  "(\<And>y. y \<in> A \<Longrightarrow> y \<le> x) \<Longrightarrow> (\<And>y. (\<And>z. z \<in> A \<Longrightarrow> z \<le> y) \<Longrightarrow> x \<le> y) \<Longrightarrow> \<Squnion>A = x"
+  apply (rule is_Sup_eq_Sup[symmetric])
+  using local.is_SupI by blast
+
+lemma SUP_diff_nat:
+  "(SUP i\<in>I. f i - c :: nat) = (SUP i\<in>I. f i) - c"
+  apply (rule antisym)
+apply (rule mono_ccSUP)
+  apply (rule Sup_eqI)
+  thm Sup_eqI
+  apply (auto intro!: SUP_eqI diff_le_mono SUP_least intro: SUP_upper
+           simp: ennreal_minus_cancel_iff ennreal_minus_le_iff less_top[symmetric])
+
+try0
+sledgehammer [dont_slice]
+by -
+
+
+lemma oracle_number_substitute_oracles_raw[simp]: \<open>oracle_number (substitute_oracles_raw os p) \<le> max (oracle_number p - length os) (\<Squnion>q\<in>set os. oracle_number q)\<close>
+proof (induction p arbitrary: os)
+  case (Seq p1 p2)
+  then show ?case
+    apply (simp add: max_diff_distrib_left_nat)
+    by (meson pre_arith_simps(3))
+next
+  case Skip
+  then show ?case
+    by simp
+next
+  case (Sample x)
+  then show ?case
+    by simp
+next
+  case (IfThenElse x1 p1 p2)
+  then show ?case 
+    apply (simp add: max_diff_distrib_left_nat)
+    by (meson pre_arith_simps(3))
+next
+  case (While x1 p)
+  then show ?case 
+    by simp
+next
+  case (QuantumOp x)
+  then show ?case
+    by simp
+next
+  case (Measurement x)
+  then show ?case 
+    by simp
+next
+  case (InstantiateOracles p x2)
+  show ?case
+  proof (cases \<open>x2 = []\<close>)
+    case True
+    then show ?thesis 
+      by (simp add: InstantiateOracles)
+  next
+    case False
+    have aux: \<open>max a (max b c) \<le> max (max d e - l) c\<close> 
+      if \<open>a \<le> d - l\<close> and \<open>b \<le> max (e - l) c\<close>
+      for a b c d e f l :: nat
+      by x
+    have \<open>oracle_number (substitute_oracles_raw os (InstantiateOracles p x2)) \<le> 
+      max (oracle_number p - length (map (substitute_oracles_raw os) x2 @ os))
+        (\<Squnion>a\<in>set (map (substitute_oracles_raw os) x2 @ os). oracle_number a)\<close>
+      using InstantiateOracles.IH(1)[where os=\<open>map (substitute_oracles_raw os) x2 @ os\<close>]
+      by simp
+    also have \<open>\<dots> = max (oracle_number p - length (map (substitute_oracles_raw os) x2 @ os)) 
+               (max (\<Squnion>a\<in>set x2. oracle_number (substitute_oracles_raw os a)) (\<Squnion>a\<in>set os. oracle_number a))\<close>
+      apply (cases \<open>x2 = []\<close>; cases \<open>os = []\<close>)
+      by (auto simp: image_image cSUP_union sup_max)
+    also have \<open>\<dots> \<le> max (max (oracle_number p - length x2) (\<Squnion>x\<in>set x2. oracle_number x) - length os) (\<Squnion>a\<in>set os. oracle_number a)\<close>
+    proof (rule aux)
+      show \<open>oracle_number p - length (map (substitute_oracles_raw os) x2 @ os) \<le> oracle_number p - length x2 - length os\<close>
+        by simp
+      have \<open>(\<Squnion>a\<in>set x2. oracle_number (substitute_oracles_raw os a)) 
+              \<le> (\<Squnion>a\<in>set x2. max (oracle_number a - length os) (\<Squnion>a\<in>set os. oracle_number a))\<close>
+        apply (cases \<open>x2 = []\<close>)
+        using InstantiateOracles(2)
+        by (auto intro!: cSUP_mono)
+      also have \<open>\<dots> = max (\<Squnion>a\<in>set x2. oracle_number a - length os) (\<Squnion>a\<in>set x2. \<Squnion>a\<in>set os. oracle_number a)\<close>
+        apply (cases \<open>x2 = []\<close>)
+        apply simp
+        apply (simp only: flip: sup_max)
+        apply (subst SUP_sup_distrib)
+        by auto
+      also have \<open>\<dots> \<le> max ((\<Squnion>x\<in>set x2. oracle_number x) - length os) (\<Squnion>a\<in>set os. oracle_number a)\<close>
+        apply (cases \<open>x2 = []\<close>, simp)
+        apply (rule max.mono)
+        try0
+        apply auto
+        sledgehammer [dont_slice]
+        by -
+        
+      finally show \<open>(\<Squnion>a\<in>set x2. oracle_number (substitute_oracles_raw os a)) \<le> max ((\<Squnion>x\<in>set x2. oracle_number x) - length os) (\<Squnion>a\<in>set os. oracle_number a)\<close>
+        by -
+      by x
+    also have \<open>\<dots> = max (oracle_number (InstantiateOracles p x2) - length os) (\<Squnion>a\<in>set os. oracle_number a)\<close>
+      by simp
+  
+  
+  also have \<open>\<dots> \<le> max (oracle_number (InstantiateOracles p x2) - length os)
+        (\<Squnion>a\<in>set (map (substitute_oracles_raw os) x2 @ os). oracle_number a)\<close>
+    apply (rule max.mono[OF _ order.refl])
+    by simp
+  also have \<open>\<dots> \<le> max (oracle_number (InstantiateOracles p x2) - length os) (\<Squnion>a\<in>set os. oracle_number a)\<close>
+  proof (rule max.mono[OF order.refl], cases \<open>x2 = []\<close>)
+    case True
+    then show \<open>(\<Squnion>a\<in>set (map (substitute_oracles_raw os) x2 @ os). oracle_number a) \<le> (\<Squnion>a\<in>set os. oracle_number a)\<close>
+      by simp
+  next
+    case False
+    have \<open>(\<Squnion>a\<in>set (map (substitute_oracles_raw os) x2 @ os). oracle_number a)
+           = max \<close>
+    apply (auto intro!: simp: )
+    try0
+sledgehammer [dont_slice]
+by -
+  also have \<open>\<dots> \<le> (\<Squnion>a\<in>set os. oracle_number a)\<close>
+    apply (rule max.boundedI[OF _ order.refl])
+  proof (rule cSUP_least)
+    show \<open>set x2 \<noteq> {}\<close>
+      using False by simp
+    fix x assume \<open>x \<in> set x2\<close>
+    show \<open>oracle_number (substitute_oracles_raw os x) \<le> (\<Squnion>a\<in>set os. oracle_number a)\<close>
+      using InstantiateOracles.IH(2)[where os=os, OF \<open>x \<in> set x2\<close>]
+try0
+sledgehammer [dont_slice]
+by -
+qed
+  finally    show \<open>(\<Squnion>a\<in>set (map (substitute_oracles_raw os) x2 @ os). oracle_number a) \<le> (\<Squnion>a\<in>set os. oracle_number a)\<close> 
+    by -
+qed
+  finally show ?case
+    by -
+next
+  case (LocalQ x1 x2 p)
+  then show ?case 
+    by simp
+next
+  case (LocalC x1 x2 p)
+  then show ?case 
+    by simp
+next
+  case (OracleCall x)
+  show ?case 
+    by (auto intro!: le_cSup_finite)
+qed
+
+lemma no_oracles_substitute_oracles_raw:
+  assumes \<open>oracle_number p = 0\<close>
+  shows \<open>no_oracles (substitute_oracles_raw p)\<close>
+  sorry
+
+lemma substitute_oracles_raw_no_oracles:
+  assumes \<open>no_oracles p\<close>
+  shows \<open>substitute_oracles_raw p = p\<close>
+  sorry
+
 
 
 inductive valid_oracle_program :: \<open>raw_program \<Rightarrow> bool\<close> and valid_program :: \<open>raw_program \<Rightarrow> bool\<close> where
@@ -81,6 +291,26 @@ inductive valid_oracle_program :: \<open>raw_program \<Rightarrow> bool\<close> 
 | \<open>valid_oracle_program c \<Longrightarrow> ACTUAL_QREGISTER q \<Longrightarrow> norm \<rho> = 1 \<Longrightarrow> valid_oracle_program (LocalQ q \<rho> c)\<close>
 | \<open>valid_oracle_program c \<Longrightarrow> ACTUAL_CREGISTER x \<Longrightarrow> valid_oracle_program (LocalC x init c)\<close>
 | \<open>valid_oracle_program c \<Longrightarrow> no_oracles c \<Longrightarrow> valid_program c\<close>
+
+lemma valid_oracle_program_substitute_oracles_raw[intro]:
+  assumes \<open>valid_oracle_program p\<close>
+  shows \<open>valid_oracle_program (substitute_oracles_raw p)\<close>
+  sorry
+
+
+lemma valid_program_substitute_oracles_raw[intro]:
+  assumes \<open>valid_oracle_program p\<close> and \<open>oracle_number p = 0\<close>
+  shows \<open>valid_program (substitute_oracles_raw p)\<close>
+  using assms(1) assms(2) no_oracles_substitute_oracles_raw valid_oracle_program_valid_program.intros(11) by blast
+
+  
+
+lemma valid_program_LocalQ: \<open>valid_program c \<Longrightarrow> ACTUAL_QREGISTER q \<Longrightarrow> norm \<rho> = 1 \<Longrightarrow> valid_program (LocalQ q \<rho> c)\<close>
+  by (meson no_oracles.simps(4) valid_oracle_program_valid_program.intros(11) valid_oracle_program_valid_program.intros(9) valid_program.cases)
+
+
+lemma valid_program_LocalC: \<open>valid_program c \<Longrightarrow> ACTUAL_CREGISTER x \<Longrightarrow> valid_program (LocalC x init c)\<close>
+  by (simp add: valid_oracle_program_valid_program.intros(10) valid_program.simps)
 
 
 typedef program = \<open>Collect valid_program\<close>
@@ -173,11 +403,35 @@ definition while :: \<open>bool expression \<Rightarrow> program list \<Rightarr
 (* lift_definition qinit :: \<open>'a qvariable \<Rightarrow> 'a ell2 expression \<Rightarrow> program\<close> is
 \<open>\<lambda>... QuantumOp\<close> *)
 
+lemma actual_cregister_range_empty[iff]: \<open>actual_cregister_range empty_cregister_range\<close>
+proof (intro actual_cregister_range_def[THEN iffD2] conjI allI)
+  show \<open>valid_cregister_range empty_cregister_range\<close>
+  using valid_empty_cregister_range by blast
+  fix m m' :: 'a
+  show \<open>\<exists>a\<in>empty_cregister_range. \<exists>b\<in>map_commutant empty_cregister_range. (a \<circ>\<^sub>m b) m = Some m'\<close>
+    apply (rule bexI[of _ Some, rotated])
+     apply (simp add: empty_cregister_range_def)
+    apply (rule bexI[of _ \<open>\<lambda>_. Some m'\<close>])
+    by simp_all
+qed
+
+lemma ACTUAL_CREGISTER_CREGISTER_of[iff]: \<open>ACTUAL_CREGISTER (CREGISTER_of F)\<close>
+  apply (cases \<open>cregister F\<close>)
+   apply (simp add: ACTUAL_CREGISTER.rep_eq CREGISTER_of.rep_eq actual_register_range)
+  by (simp add: non_cregister ACTUAL_CREGISTER.rep_eq bot_CREGISTER.rep_eq)
+
+
+lift_definition localvars1 :: "'a cvariable \<Rightarrow> 'b qvariable \<Rightarrow> program \<Rightarrow> program" is
+  \<open>\<lambda>C Q p. LocalC (CREGISTER_of C) undefined (LocalQ (QREGISTER_of Q) (tc_butterfly (ket undefined) (ket undefined)) p)\<close>
+  by (auto intro!: valid_program_LocalC valid_program_LocalQ ACTUAL_QREGISTER_QREGISTER_of simp: norm_tc_butterfly)
+
+definition localvars :: "'a cvariable \<Rightarrow> 'b qvariable \<Rightarrow> program list \<Rightarrow> program" where
+  \<open>localvars C Q ps = localvars1 C Q (block ps)\<close>
+
 consts
   qinit :: "'a qvariable \<Rightarrow> 'a ell2 expression \<Rightarrow> program"
   measurement :: "'a cvariable \<Rightarrow> 'b qvariable \<Rightarrow> ('a,'b) measurement expression \<Rightarrow> program"
   instantiateOracles :: "oracle_program \<Rightarrow> program list \<Rightarrow> program"
-  localvars :: "'a cvariable \<Rightarrow> 'b qvariable \<Rightarrow> program list \<Rightarrow> program"
 
 (* fun fvq_raw_program :: \<open>raw_program \<Rightarrow> QVARIABLE\<close> where
   \<open>fvq_raw_program (Seq p q) = fvq_raw_program p \<squnion> fvq_raw_program q\<close>
@@ -194,7 +448,10 @@ consts
 
 
 lemma localvars_empty: "localvars empty_cregister empty_qregister P = block P"
-  sorry
+(* TODO: not true with current definition. Only denotationally equal.
+Do we need this lemma? If yes, we can change the definition of localvars to skip the LocalC/LocalQ for one_dim_algebras. *)
+apply (auto intro!: Rep_program_inject[THEN iffD1] simp add: localvars_def localvars1.rep_eq)
+  thm Rep_program_inject  sorry
 
 
 (* definition \<open>swap_QREGISTER' = (\<lambda>(f,U,L,R).
@@ -310,9 +567,34 @@ lemma denotation_sample: \<open>denotation (sample x e) = cq_map_sample (\<lambd
   apply (transfer' fixing: x e)
   by simp
 
-(* TODO nicer one *)
-lemma denotation_assign: \<open>denotation (assign x e) = cq_map_sample (\<lambda>m. point_distr (Classical_Registers.setter x (e m) m))\<close>
+lemma kraus_family_norm_sample_prob: \<open>kraus_family_norm (kraus_map_sample (prob \<mu>) :: ('a::{chilbert_space,not_singleton},'a,'x) kraus_family) = weight \<mu>\<close>
+  apply (subst kraus_map_sample_norm[of \<open>prob \<mu>\<close>])
+  by (auto intro!: prob_summable simp: Prob.rep_eq)
+
+lemma kraus_map_sample_point_distr': \<open>kraus_family_remove_0 (kraus_map_sample (prob (point_distr x))) = kraus_family_remove_0 (kraus_family_map_outcome_inj (\<lambda>_. x) kraus_family_id)\<close>
+  apply (rule Rep_kraus_family_inject[THEN iffD1])
+  by (auto intro!: prob_summable
+      simp: kraus_map_sample.rep_eq kraus_family_map_outcome_inj.rep_eq kraus_family_id_def
+      kraus_family_of_op.rep_eq kraus_family_remove_0.rep_eq image_iff)
+
+lemma kraus_map_sample_point_distr: \<open>kraus_equivalent' (kraus_map_sample (prob (point_distr x))) (kraus_family_map_outcome_inj (\<lambda>_. x) kraus_family_id)\<close>
+  using kraus_map_sample_point_distr'[of x] kraus_family_remove_0_equivalent'
+    kraus_equivalent'_sym kraus_equivalent'_trans
+  by metis
+
+lemma cq_map_eqI:
+  assumes \<open>cq_map_rel (rep_cq_map E) (rep_cq_map F)\<close>
+  shows \<open>E = F\<close>
+  using assms Quotient3_cq_map Quotient3_rel_rep by fastforce
+
+lemma cq_map_sample_point_distr: \<open>cq_map_sample (\<lambda>x. point_distr (f x)) = cq_map_classical f\<close>
+  apply (transfer' fixing: )
+  by (auto intro!: kraus_map_sample_point_distr simp: cq_map_rel_def kraus_family_norm_sample_prob)
+
+lemma denotation_assign_sample: \<open>denotation (assign x e) = cq_map_sample (\<lambda>m. point_distr (Classical_Registers.setter x (e m) m))\<close>
   by (simp add: assign_def denotation_sample)
+lemma denotation_assign: \<open>denotation (assign x e) = cq_map_classical (\<lambda>m. Classical_Registers.setter x (e m) m)\<close>
+  by (simp add: denotation_assign_sample cq_map_sample_point_distr)
 
 lemma denotation_skip: \<open>denotation skip = cq_map_id\<close>
   apply transfer' 
@@ -336,6 +618,16 @@ next
     by (simp add: block_cons denotation_seq)
 qed
 
+lemma denotation_ifthenelse1:
+  \<open>denotation (ifthenelse1 c p q) = cq_map_if c (denotation p) (denotation q)\<close>
+  apply (transfer' fixing: c)
+  by simp
+
+lemma denotation_ifthenelse:
+  \<open>denotation (ifthenelse c p q) = cq_map_if c (denotation (block p)) (denotation (block q))\<close>
+  by (simp add: denotation_ifthenelse1 ifthenelse_def)
+
+
 lift_definition kraus_family_in_qref_strict :: \<open>('qu ell2,'qu ell2,'cl) kraus_family \<Rightarrow> 'qu QREGISTER \<Rightarrow> bool\<close> is
   \<open>\<lambda>\<EE> Q. \<forall>(E,x)\<in>\<EE>. E \<in> Rep_QREGISTER Q\<close>.
 definition kraus_family_in_qref :: \<open>('qu ell2,'qu ell2,'cl) kraus_family \<Rightarrow> 'qu QREGISTER \<Rightarrow> bool\<close> where
@@ -347,11 +639,22 @@ lift_definition qc_map_in_qref :: \<open>('cl1,'qu,'cl2,'qu) cq_map \<Rightarrow
   using kraus_equivalent'_trans kraus_equivalent'_sym
   by meson
 
-definition fvq_of_cq_map :: \<open>(cl, qu, cl, qu) cq_map \<Rightarrow> QVARIABLE\<close> where
-  \<open>fvq_of_cq_map \<EE> = Inf {Q. qc_map_in_qref \<EE> Q}\<close>
+(* definition fvq_of_cq_map :: \<open>(cl, qu, cl, qu) cq_map \<Rightarrow> QVARIABLE\<close> where
+  \<open>fvq_of_cq_map \<EE> = Inf {Q. qc_map_in_qref \<EE> Q}\<close> *)
 
-definition fvq_program :: \<open>program \<Rightarrow> QVARIABLE\<close> where
-  \<open>fvq_program p = fvq_of_cq_map (denotation p)\<close>
+definition program_in_qref :: \<open>program \<Rightarrow> QVARIABLE \<Rightarrow> bool\<close> where
+  \<open>program_in_qref p = qc_map_in_qref (denotation p)\<close>
+
+(* definition fvq_program :: \<open>program \<Rightarrow> QVARIABLE\<close> where
+  \<open>fvq_program p = fvq_of_cq_map (denotation p)\<close> *)
+
+inductive raw_program_in_qref :: \<open>raw_program \<Rightarrow> QVARIABLE \<Rightarrow> bool\<close> where
+  \<open>no_oracles p \<Longrightarrow> qc_map_in_qref (denotation_raw p) Q \<Longrightarrow> raw_program_in_qref p Q\<close>
+| \<open>raw_program_in_qref p Q \<Longrightarrow> raw_program_in_qref q Q \<Longrightarrow> raw_program_in_qref (Seq p q) Q\<close>
+| \<open>raw_program_in_qref p Q \<Longrightarrow> raw_program_in_qref q Q \<Longrightarrow> raw_program_in_qref (IfThenElse c p q) Q\<close>
+| \<open>raw_program_in_qref p Q \<Longrightarrow> raw_program_in_qref (While c p) Q\<close>
+| \<open>fvq_raw_program (InstantiateOracles p qs) = fvq_raw_program p \<squnion> (\<Squnion>q\<in>set qs. fvq_raw_program q)\<close>
+
 
 function fvq_raw_program :: \<open>raw_program \<Rightarrow> QVARIABLE\<close> where
  \<open>no_oracles p \<Longrightarrow> fvq_raw_program p = fvq_of_cq_map (denotation_raw p)\<close>
@@ -371,8 +674,70 @@ consts fvcw_program :: "program \<Rightarrow> CVARIABLE"
 consts fvc_oracle_program :: "oracle_program \<Rightarrow> CVARIABLE"
 consts fvcw_oracle_program :: "oracle_program \<Rightarrow> CVARIABLE"
 
+lemma kraus_family_in_qref_strict_map:
+  assumes \<open>kraus_family_in_qref_strict \<EE> Q\<close>
+  shows \<open>kraus_family_in_qref_strict (kraus_family_map_outcome f \<EE>) Q\<close>
+proof -
+  have \<open>E \<in> Rep_QREGISTER Q\<close> if \<open>(E,x) \<in> Rep_kraus_family (kraus_family_map_outcome f \<EE>)\<close> for E x
+  proof -
+    from that
+    have \<open>(norm E)\<^sup>2 = kraus_family_op_weight (kraus_family_filter (\<lambda>y. f y = x) \<EE>) E\<close> and \<open>E \<noteq> 0\<close>
+      by (simp_all add: kraus_family_map_outcome.rep_eq)
+    then have \<open>kraus_family_op_weight (kraus_family_filter (\<lambda>y. f y = x) \<EE>) E \<noteq> 0\<close>
+      by auto
+    then have \<open>(\<Sum>\<^sub>\<infinity>(F,_)\<in>kraus_family_related_ops (kraus_family_filter (\<lambda>y. f y = x) \<EE>) E. norm (F* o\<^sub>C\<^sub>L F)) \<noteq> 0\<close>
+      by (simp add: kraus_family_op_weight_def)
+    then have \<open>kraus_family_related_ops (kraus_family_filter (\<lambda>y. f y = x) \<EE>) E \<noteq> {}\<close>
+      by force
+    then obtain F y r where \<open>(F,y) \<in> Rep_kraus_family (kraus_family_filter (\<lambda>y. f y = x) \<EE>)\<close> and \<open>E = r *\<^sub>R F\<close>
+      by (auto simp add: kraus_family_related_ops_def)
+    then have \<open>(F,y) \<in> Rep_kraus_family \<EE>\<close>
+      by (simp add: kraus_family_filter.rep_eq)
+    with assms have \<open>F \<in> Rep_QREGISTER Q\<close>
+      by (metis (no_types, lifting) case_prodE fst_conv kraus_family_in_qref_strict.rep_eq)
+    with \<open>E = r *\<^sub>R F\<close> show \<open>E \<in> Rep_QREGISTER Q\<close>
+      using Rep_QREGISTER[of Q]
+      by (auto intro!: complex_vector.subspace_scale
+          simp: scaleR_scaleC valid_qregister_range_def von_neumann_algebra_def_sot)
+  qed
+  then show ?thesis
+    by (force simp: kraus_family_in_qref_strict.rep_eq)
+qed
+
+
+lemma kraus_family_in_qref_map:
+  assumes \<open>kraus_family_in_qref \<EE> Q\<close>
+  shows \<open>kraus_family_in_qref (kraus_family_map_outcome f \<EE>) Q\<close>
+proof -
+  from assms
+  obtain \<FF> where eq: \<open>kraus_equivalent' \<EE> \<FF>\<close> and qref: \<open>kraus_family_in_qref_strict \<FF> Q\<close>
+    by (auto simp: kraus_family_in_qref_def)
+  define \<FF>' where \<open>\<FF>' = kraus_family_map_outcome f \<FF>\<close>
+  have eq': \<open>kraus_equivalent' (kraus_family_map_outcome f \<EE>) \<FF>'\<close>
+    by (simp add: \<FF>'_def eq kraus_equivalent'_map_cong)
+  have qref': \<open>kraus_family_in_qref_strict \<FF>' Q\<close>
+    using qref[THEN kraus_family_in_qref_strict_map]
+    by (auto simp: \<FF>'_def )
+  from eq' qref' show \<open>kraus_family_in_qref (kraus_family_map_outcome f \<EE>) Q\<close>
+    by (auto intro!: exI[of _ \<FF>'] simp add: kraus_family_in_qref_def)
+qed
+
+lemma kraus_family_in_qref_strict_id[iff]: \<open>kraus_family_in_qref_strict kraus_family_id Q\<close>
+  using Rep_QREGISTER valid_qregister_range_def_sot
+  by (auto intro!: simp: kraus_family_id_def  kraus_family_of_op.rep_eq kraus_family_in_qref_strict_def)
+
+lemma kraus_family_in_qref_id[iff]: \<open>kraus_family_in_qref kraus_family_id Q\<close>
+  by (auto intro!: exI[of _ kraus_family_id] simp: kraus_family_in_qref_def)
+
+lemma qc_map_in_qref_id[iff]: \<open>qc_map_in_qref cq_map_id Q\<close>
+  apply (transfer fixing: Q)
+  by (auto intro!: kraus_family_in_qref_map)
+
+lemma fvq_of_cq_map_id[iff]: \<open>fvq_of_cq_map cq_map_id = \<bottom>\<close>
+  by (simp add: fvq_of_cq_map_def)
+
 lemma fvq_program_skip[simp]: \<open>fvq_program skip = \<bottom>\<close>
-  sorry
+  by (auto intro!: simp: fvq_program_def denotation_skip)
 
 (* TODO Truth is \<le> *)
 lemma fvq_program_seq: \<open>fvq_program (seq a b) = fvq_program a \<squnion> fvq_program b\<close>
@@ -403,14 +768,115 @@ next
     by (simp add: yzs_def)
 qed
 
+
+lemma kraus_family_in_qref_strict_sample[iff]: \<open>kraus_family_in_qref_strict (kraus_map_sample f) Q\<close>
+  using Rep_QREGISTER[of Q]
+  by (auto intro!:complex_vector.subspace_scale
+      simp: valid_qregister_range_def_sot scaleR_scaleC kraus_map_sample.rep_eq kraus_family_in_qref_strict_def)
+
+lemma kraus_family_in_qref_sample[iff]: \<open>kraus_family_in_qref (kraus_map_sample f) Q\<close>
+  by (auto intro!: exI[of _ \<open>kraus_map_sample f\<close>] simp: kraus_family_in_qref_def)
+
+lemma qc_map_in_qref_sample[iff]: \<open>qc_map_in_qref (cq_map_sample f) Q\<close>
+  apply (transfer fixing: Q)
+  by (auto intro!: kraus_family_in_qref_map)
+
+lemma fvq_of_cq_map_sample[simp]: \<open>fvq_of_cq_map (cq_map_sample f) = \<bottom>\<close>
+  by (simp add: fvq_of_cq_map_def)
+
 lemma fvq_program_sample: "fvq_program (sample xs e2) = QREGISTER_unit"
-  sorry
+  by (simp add: fvq_program_def denotation_sample)
 lemma fvq_program_assign: "fvq_program (assign x e) = QREGISTER_unit"
-  sorry
-(* TODO Truth is \<le> *)
-lemma fvq_program_ifthenelse: "fvq_program (ifthenelse c p1 p2) =
+  by (simp add: fvq_program_def denotation_assign_sample)
+
+lemma kraus_family_in_qref_top[iff]: \<open>kraus_family_in_qref E \<top>\<close>
+  by (auto intro!: exI[of _ E] simp add: kraus_family_in_qref_def kraus_family_in_qref_strict_def top_QREGISTER.rep_eq)
+
+lemma
+  assumes \<open>\<close>
+  shows \<open>qc_map_in_qref (cq_map_if c E F) Q\<close>
+
+lemma fvq_of_cq_map_if: \<open>fvq_of_cq_map (cq_map_if c E F) \<le> fvq_of_cq_map E \<squnion> fvq_of_cq_map F\<close>
+
+  by xxx
+proof (unfold fvq_of_cq_map_def, transfer' fixing: c)
+  fix E F :: \<open>cl \<Rightarrow> (qu ell2, qu ell2, cl) kraus_family\<close>
+
+  have aux: \<open>A \<subseteq> commutant (commutant B)\<close> if \<open>A \<subseteq> B\<close> for A B
+try0
+sledgehammer [dont_slice]
+  using double_commutant_grows that by blast
+by -
+
+
+  show \<open>\<Sqinter> {Q. \<forall>x. kraus_family_in_qref (if c x then E x else F x) Q}
+           \<le> \<Sqinter> {Q. \<forall>x. kraus_family_in_qref (E x) Q} \<squnion> \<Sqinter> {Q. \<forall>x. kraus_family_in_qref (F x) Q}\<close>
+    apply (simp add: less_eq_QREGISTER_def Inf_QREGISTER.rep_eq sup_QREGISTER.rep_eq)
+    apply (rule aux)
+    apply (auto intro!: simp: )
+try0
+sledgehammer [dont_slice]
+by -
+
+apply (transfer' fixing: )
+
+    
+    
+    by -
+
+
+
+  have \<open>\<Sqinter> {Q. \<forall>x. kraus_family_in_qref (if c x then E x else F x) Q}
+\<le> \<Sqinter> {Q. \<forall>x. kraus_family_in_qref (E x) Q \<or> kraus_family_in_qref (F x) Q}\<close>
+apply (rule Inf_superset_mono)
+try0
+sledgehammer [dont_slice]
+by -
+  also have \<open>\<dots> \<le> \<Sqinter> {Q. \<forall>x. kraus_family_in_qref (E x) Q} \<squnion> \<Sqinter> {Q. \<forall>x. kraus_family_in_qref (F x) Q}\<close>
+  by (simp add: Inf_superset_mono Set.basic_monos(6) sup.coboundedI2)
+  finally 
+  show \<open>\<Sqinter> {Q. \<forall>x. kraus_family_in_qref (if c x then E x else F x) Q}
+           \<le> \<Sqinter> {Q. \<forall>x. kraus_family_in_qref (E x) Q} \<squnion> \<Sqinter> {Q. \<forall>x. kraus_family_in_qref (F x) Q}\<close>
+    by -
+
+
+  proof (rule Inf_less_eq, rename_tac Q)
+    show \<open>{Q. \<forall>x. kraus_family_in_qref (if c x then E x else F x) Q} \<noteq> {}\<close>
+      by (auto intro!: exI[of _ \<top>])
+    fix Q assume asm: \<open>Q \<in> {Q. \<forall>x. kraus_family_in_qref (if c x then E x else F x) Q}\<close>
+    then have \<open>kraus_family_in_qref (E x) Q\<close> if \<open>c x\<close> for x
+      using that by (smt (verit, ccfv_threshold) mem_Collect_eq)
+    moreover from asm have \<open>kraus_family_in_qref (F x) Q\<close> if \<open>\<not> c x\<close> for x
+      by (smt (verit, ccfv_SIG) mem_Collect_eq that)
+    ultimately have \<open>Q \<le> \<Sqinter> {Q. \<forall>x. kraus_family_in_qref (E x) Q \<or> kraus_family_in_qref (F x) Q}\<close>
+apply (auto intro!: Inf_greatest simp: )
+try0
+sledgehammer [dont_slice]
+by -
+  also have \<open>\<dots> \<le> \<Sqinter> {Q. \<forall>x. kraus_family_in_qref (E x) Q} \<squnion> \<Sqinter> {Q. \<forall>x. kraus_family_in_qref (F x) Q}\<close>
+  by (simp add: Inf_superset_mono Set.basic_monos(6) sup.coboundedI2)
+by -
+
+
+  have \<open>\<Sqinter> {Q. \<forall>x. kraus_family_in_qref (E x) Q} \<squnion> \<Sqinter> {Q. \<forall>x. kraus_family_in_qref (F x) Q}
+      = (\<Sqinter>x. Collect (kraus_family_in_qref (E x))) \<squnion> (\<Sqinter>x. Collect (kraus_family_in_qref (F x)))\<close>
+try0
+sledgehammer [dont_slice]
+by -
+
+    show \<open>Q \<le> \<Sqinter> {Q. \<forall>x. kraus_family_in_qref (E x) Q} \<squnion> \<Sqinter> {Q. \<forall>x. kraus_family_in_qref (F x) Q}\<close>
+
+  apply (auto intro!: simp: fvq_of_cq_map_def)
+  apply (transfer' fixing: )
+apply (auto intro!: Inf_less_eq simp: )
+
+  by x
+lemma fvq_program_ifthenelse1: "fvq_program (ifthenelse1 c p1 p2) \<le>
+  QREGISTER_pair (fvq_program p1) (fvq_program p2)"
+  by (auto intro!: fvq_of_cq_map_if simp: fvq_program_def denotation_ifthenelse1)
+lemma fvq_program_ifthenelse: "fvq_program (ifthenelse c p1 p2) \<le>
   QREGISTER_pair (fvq_program (block p1)) (fvq_program (block p2))"
-  sorry
+  using fvq_program_ifthenelse1 ifthenelse_def by presburger
 (* TODO Truth is \<le> *)
 lemma fvq_program_while: "fvq_program (while c b) = (fvq_program (block b))"
   sorry
